Runwai/Command.lean
@@ -52,8 +52,8 @@ unsafe def elabLodaProve : Elab.Command.CommandElab
 
     -- Generate the theorem syntax
     let theoremStx ← `(command|
-      theorem $theoremIdent (Δ: Env.ChipEnv) (h_delta: Δ = $deltaTerm) : (Ty.ChipCorrect $deltaTerm $circTerm 1) := by
-        (unfold Ty.ChipCorrect; intro x i hs hi hrow ht hσ; set envs := Ty.makeEnvs $circTerm (Ast.Value.vArr x) (Ast.Value.vZ i) x.length);
+      theorem $theoremIdent (Δ: Env.ChipEnv) (h_delta: Δ = $deltaTerm) : (Ty.chipCorrect $deltaTerm $circTerm 1) := by
+        (unfold Ty.chipCorrect; intro x i hs hi hrow ht hσ; set envs := Ty.makeEnvs $circTerm (Ast.Value.vArr x) (Ast.Value.vZ i) x.length);
         (set σ := envs.1); (set Γ := envs.2); ($proof);
     )
     logInfo m!"Proof state opened for '{theoremName}' - continue with tactics!"
